Extend the frontend language with break/continue, named variables, and static variables.

frontend.v
@@ -4,14 +4,13 @@ Require Import type_system expression_eval.
 Local Open Scope expr_scope.
 Local Open Scope ctype_scope.
 
-Inductive cexpr (Ti : Set) :=
-  | EVar : nat → cexpr Ti
-  | EGlob : nat → cexpr Ti
+Inductive cexpr (Ti : Set) : Set :=
+  | EVar : N → cexpr Ti
   | EConst : int_type Ti → Z → cexpr Ti
   | EAddrOf : cexpr Ti → cexpr Ti
   | EDeref : cexpr Ti → cexpr Ti
   | EAssign : assign → cexpr Ti → cexpr Ti → cexpr Ti
-  | ECall : funname → list (cexpr Ti) → cexpr Ti
+  | ECall : N → list (cexpr Ti) → cexpr Ti
   | EAlloc : type Ti → cexpr Ti
   | EFree : cexpr Ti → cexpr Ti
   | EUnOp : unop → cexpr Ti → cexpr Ti
@@ -21,7 +20,6 @@ Inductive cexpr (Ti : Set) :=
   | ECast : type Ti → cexpr Ti → cexpr Ti
   | EField : cexpr Ti → nat → cexpr Ti.
 Arguments EVar {_} _.
-Arguments EGlob {_} _.
 Arguments EConst {_} _ _.
 Arguments EAddrOf {_} _.
 Arguments EDeref {_} _.
@@ -36,14 +34,15 @@ Arguments EComma {_} _ _.
 Arguments ECast {_} _ _.
 Arguments EField {_} _ _.
 
-Inductive cstmt (Ti : Set) :=
+Inductive cstmt (Ti : Set) : Set :=
   | SDo : cexpr Ti → cstmt Ti
   | SSkip : cstmt Ti
   | SGoto : labelname → cstmt Ti
   | SBreak : cstmt Ti
   | SContinue : cstmt Ti
   | SReturn : option (cexpr Ti) → cstmt Ti
-  | SBlock : type Ti → cstmt Ti → cstmt Ti
+  | SBlock : N → type Ti → option (cexpr Ti) → cstmt Ti → cstmt Ti
+  | SStatic : N → type Ti → option (cexpr Ti) → cstmt Ti → cstmt Ti
   | SComp : cstmt Ti → cstmt Ti → cstmt Ti
   | SLabel : labelname → cstmt Ti → cstmt Ti
   | SWhile : cexpr Ti → cstmt Ti → cstmt Ti
@@ -54,25 +53,38 @@ Arguments SGoto {_} _.
 Arguments SBreak {_}.
 Arguments SContinue {_}.
 Arguments SReturn {_} _.
-Arguments SBlock {_} _ _.
+Arguments SBlock {_} _ _ _ _.
+Arguments SStatic {_} _ _ _ _.
 Arguments SComp {_} _ _.
 Arguments SLabel {_} _ _.
 Arguments SWhile {_} _ _.
 Arguments SIf {_} _ _ _.
 
-Record cenv (Ti : Set) := CEnv {
-  c_env : list (tag * list (type Ti));
-  c_globals : list (type Ti * option (cexpr Ti));
-  c_funs : list (funname * list (type Ti) * type Ti * cstmt Ti)
-}.
-Arguments CEnv {_} _ _ _.
-Arguments c_env {_} _.
-Arguments c_globals {_} _.
-Arguments c_funs {_} _.
+Inductive decl (Ti : Set) : Set :=
+  | CompoundDecl : list (type Ti) → decl Ti
+  | GlobDecl : type Ti → option (cexpr Ti) → decl Ti
+  | FunDecl : list (N * type Ti) → type Ti → cstmt Ti → decl Ti.
+Arguments CompoundDecl {_} _.
+Arguments GlobDecl {_} _ _.
+Arguments FunDecl {_} _ _ _.
+
+Notation var_env Ti := (list (N * (index + type Ti))).
 
 Section frontend.
 Context `{IntEnv Ti, PtrEnv Ti}.
 
+Fixpoint lookup_var (m : mem Ti) (x : N)
+    (i : nat) (xs : var_env Ti) : option (expr Ti * type Ti) :=
+  match xs with
+  | [] => None
+  | (y,inl o) :: xs =>
+     if decide (x = y)
+     then τ ← type_check m o; Some (% (addr_top o τ), τ)
+     else lookup_var m x i xs
+  | (y,inr τ) :: xs =>
+     if decide (x = y) then Some (var{τ} i, τ)
+     else lookup_var m x (S i) xs
+  end.
 Definition to_R (eτlr : expr Ti * lrtype Ti) : expr Ti * type Ti :=
   match eτlr with
   | (e, inl τ) =>
@@ -82,185 +94,224 @@ Definition to_R (eτlr : expr Ti * lrtype Ti) : expr Ti * type Ti :=
   | (e, inr τ) => (e,τ)
   end%E.
 Definition to_expr (Γ : env Ti) (Γf : funtypes Ti) (m : mem Ti)
-    (τs : list (type Ti)) : cexpr Ti → option (expr Ti * lrtype Ti) :=
-  fix go e :=
-  match e with
-  | EVar n =>
-     τ ← τs !! n;
-     Some (var{τ} n, inl τ)
-  | EGlob n =>
-     τ ← type_check m (N.of_nat n : index);
-     Some (% (addr_top (N.of_nat n) τ), inl τ)
+    (xs : var_env Ti) : cexpr Ti → option (expr Ti * lrtype Ti) :=
+  fix go ce :=
+  match ce with
+  | EVar x =>
+     '(e,τ) ← lookup_var m x 0 xs; Some (e, inl τ)
   | EConst τi x =>
      guard (int_typed x τi);
      Some (# (intV{τi} x), inr (intT τi))
-  | EDeref e =>
-     '(e',τ) ← to_R <$> go e;
+  | EDeref ce =>
+     '(e,τ) ← to_R <$> go ce;
      τp ← maybe_TBase τ ≫= maybe_TPtr;
-     Some (.* e', inl τp)
-  | EAddrOf e =>
-     '(e',τlr) ← go e;
+     Some (.* e, inl τp)
+  | EAddrOf ce =>
+     '(e,τlr) ← go ce;
      τ ← maybe_inl τlr;
-     Some (& e', inr (τ.*))
-  | EAssign ass e1 e2 =>
-     '(e1',τlr1) ← go e1;
+     Some (& e, inr (τ.*))
+  | EAssign ass ce1 ce2 =>
+     '(e1,τlr1) ← go ce1;
      τ1 ← maybe_inl τlr1;
-     '(e2',τ2) ← to_R <$> go e2;
+     '(e2,τ2) ← to_R <$> go ce2;
      σ ← assign_type_of τ1 τ2 ass;
-     Some (e1' ::={ass} e2', inr σ)
-  | ECall f es =>
-     '(τs,σ) ← Γf !! f;
-     τses ← fmap to_R <$> mapM go es;
+     Some (e1 ::={ass} e2, inr σ)
+  | ECall f ces =>
+     '(τs,σ) ← Γf !! (f : funname);
+     τses ← fmap to_R <$> mapM go ces;
      guard (snd <$> τses = τs);
      Some (call f @ fst <$> τses, inr σ)
   | EAlloc τ =>
      guard (✓{Γ} τ);
      guard (int_typed (size_of Γ τ) sptrT);
      Some (& (alloc τ), inr (τ.*))
-  | EFree e =>
-     '(e',τ) ← to_R <$> go e;
+  | EFree ce =>
+     '(e,τ) ← to_R <$> go ce;
      _ ← maybe_TBase τ ≫= maybe_TPtr;
-     Some (free (.* e'), inr voidT)
-  | EUnOp op e =>
-     '(e',τ) ← to_R <$> go e;
+     Some (free (.* e), inr voidT)
+  | EUnOp op ce =>
+     '(e,τ) ← to_R <$> go ce;
      σ ← unop_type_of op τ;
-     Some (@{op} e', inr σ)
-  | EBinOp op e1 e2 =>
-     '(e1',τ1) ← to_R <$> go e1;
-     '(e2',τ2) ← to_R <$> go e2;
+     Some (@{op} e, inr σ)
+  | EBinOp op ce1 ce2 =>
+     '(e1,τ1) ← to_R <$> go ce1;
+     '(e2,τ2) ← to_R <$> go ce2;
      σ ← binop_type_of op τ1 τ2;
-     Some (e1' @{op} e2', inr σ)
-  | EIf e1 e2 e3 =>
-     '(e1',τ1) ← to_R <$> go e1;
+     Some (e1 @{op} e2, inr σ)
+  | EIf ce1 ce2 ce3 =>
+     '(e1,τ1) ← to_R <$> go ce1;
      _ ← maybe_TBase τ1;
-     '(e2',τ2) ← to_R <$> go e2;
-     '(e3',τ3) ← to_R <$> go e3;
+     '(e2,τ2) ← to_R <$> go ce2;
+     '(e3,τ3) ← to_R <$> go ce3;
      guard (τ2 = τ3);
-     Some (if{e1'} e2' else e3', inr τ3)
-  | EComma e1 e2 =>
-     '(e1',τ1) ← to_R <$> go e1;
-     '(e2',τ2) ← to_R <$> go e2;
-     Some (e1',, e2', inr τ2)
-  | ECast σ e =>
-     '(e',τ) ← to_R <$> go e;
+     Some (if{e1} e2 else e3, inr τ3)
+  | EComma ce1 ce2 =>
+     '(e1,τ1) ← to_R <$> go ce1;
+     '(e2,τ2) ← to_R <$> go ce2;
+     Some (e1,, e2, inr τ2)
+  | ECast σ ce =>
+     '(e,τ) ← to_R <$> go ce;
      guard (cast_typed Γ τ σ);
-     Some (cast{σ} e', inr σ)
-  | EField e i =>
-     '(e',τrl) ← go e;
+     Some (cast{σ} e, inr σ)
+  | EField ce i =>
+     '(e,τrl) ← go ce;
      τ ← maybe_inl τrl;
      '(c,s) ← maybe_TCompound τ;
      σs ← Γ !! s;
      σ ← σs !! i;
-     Some (e' .> i, inl σ)
+     Some (e .> i, inl σ)
   end%E.
 
 Global Instance cstmt_labels : Labels (cstmt Ti) :=
-  fix go s := let _ : Labels _ := @go in
-  match s with
-  | SBlock _ s => labels s
-  | SComp s1 s2 => labels s1 ∪ labels s2
-  | SLabel l s => {[ l ]} ∪ labels s
-  | SWhile _ s => labels s
-  | SIf _ s1 s2 => labels s1 ∪ labels s2
+  fix go cs := let _ : Labels _ := @go in
+  match cs with
+  | SBlock _ _ _ cs | SStatic _ _ _ cs => labels cs
+  | SComp cs1 cs2 => labels cs1 ∪ labels cs2
+  | SLabel l cs => {[ l ]} ∪ labels cs
+  | SWhile _ cs => labels cs
+  | SIf _ cs1 cs2 => labels cs1 ∪ labels cs2
   | _ => ∅
   end.
-Fixpoint cstmt_has_break_continue (s : cstmt Ti) : bool :=
-  match s with
-  | SBreak | SContinue => true
-  | SBlock _ s => cstmt_has_break_continue s
-  | SComp s1 s2 => cstmt_has_break_continue s1 || cstmt_has_break_continue s2
-  | SLabel _ s => cstmt_has_break_continue s
-  | SIf _ s1 s2 => cstmt_has_break_continue s1 || cstmt_has_break_continue s2
+Fixpoint cstmt_has_continue (cs : cstmt Ti) : bool :=
+  match cs with
+  | SContinue => true
+  | SBlock _ _ _ cs | SStatic _ _ _ cs => cstmt_has_continue cs
+  | SComp cs1 cs2 => cstmt_has_continue cs1 || cstmt_has_continue cs2
+  | SLabel _ cs => cstmt_has_continue cs
+  | SIf _ cs1 cs2 => cstmt_has_continue cs1 || cstmt_has_continue cs2
   | _ => false
   end.
-Definition to_while (mLcLb : option (labelname * labelname))
-    (e : expr Ti) (s : stmt Ti) : stmt Ti :=
-  match mLcLb with
-  | Some (Lc,Lb) => while{e} (s ;; label Lc) ;; label Lb
-  | None => while{e} s
+Fixpoint cstmt_has_break (cs : cstmt Ti) : bool :=
+  match cs with
+  | SBreak => true
+  | SBlock _ _ _ cs | SStatic _ _ _ cs => cstmt_has_break cs
+  | SComp cs1 cs2 => cstmt_has_break cs1 || cstmt_has_break cs2
+  | SLabel _ cs => cstmt_has_break cs
+  | SIf _ cs1 cs2 => cstmt_has_break cs1 || cstmt_has_break cs2
+  | _ => false
   end.
 
-Definition to_stmt (Γ : env Ti) (Γf : funtypes Ti) (m : mem Ti) :
-    list (type Ti) → labelset → option (labelname * labelname) →
-    cstmt Ti → option (stmt Ti * rettype Ti) :=
-  fix go τs Ls mLcLb s {struct s} :=
-  match s with
-  | SDo e => '(e',_) ← to_R <$> to_expr Γ Γf m τs e; Some (! e', (false, None))
-  | SSkip => Some (skip, (false, None))
-  | SGoto l => Some (goto l, (true, None))
-  | SContinue => '(Lc,_) ← mLcLb; Some (goto Lc, (true, None))
-  | SBreak => '(_,Lb) ← mLcLb; Some (goto Lb, (true, None))
-  | SReturn (Some e) =>
-     '(e',τ) ← to_R <$> to_expr Γ Γf m τs e; Some (ret e', (true, Some τ))
-  | SReturn None => Some (ret (#voidV), (true, Some voidT))
-  | SBlock τ s =>
-     guard (✓{Γ} τ);
-     guard (int_typed (size_of Γ τ) sptrT);
-     '(s',cmσ) ← go (τ :: τs) Ls mLcLb s;
-     Some (blk{τ} s', cmσ)
-  | SComp s1 s2 =>
-     '(s1',cmσ1) ← go τs Ls mLcLb s1; '(s2',cmσ2) ← go τs Ls mLcLb s2;
-     mσ ← rettype_union (cmσ1.2) (cmσ2.2);
-     Some (s1' ;; s2',(cmσ2.1, mσ))
-  | SLabel l s => '(s',cmσ) ← go τs Ls mLcLb s; Some (l :; s', cmσ)
-  | SWhile e s =>
-     '(e',τ) ← to_R <$> to_expr Γ Γf m τs e; _ ← maybe_TBase τ;
-     let (mLcLr',Ls') :=
-       if cstmt_has_break_continue s
-       then let Lc := fresh Ls in let Lr := fresh ({[ Lc ]} ∪ Ls)
-            in (Some (Lc,Lr), {[ Lc ; Lr ]} ∪ Ls)
-       else (None,Ls) in
-     '(s',cmσ) ← go τs Ls' mLcLr' s; Some (to_while mLcLr' e' s',(false, cmσ.2))
-  | SIf e s1 s2 =>
-     '(e',τ) ← to_R <$> to_expr Γ Γf m τs e; _ ← maybe_TBase τ;
-     '(s1',cmσ1) ← go τs Ls mLcLb s1; '(s2',cmσ2) ← go τs Ls mLcLb s2;
-     mσ ← rettype_union (cmσ1.2) (cmσ2.2);
-     Some (if{e'} s1' else s2', (cmσ1.1 && cmσ2.1, mσ))%S
-  end%T.
-Definition to_mem (Γ : env Ti) :
-    list (type Ti  * option (cexpr Ti)) → index → mem Ti → option (mem Ti) :=
-  fix go G o m_acc :=
-  match G with
-  | [] => Some m_acc
-  | (τ,Some e) :: G =>
-     '(e',τ') ← to_R <$> to_expr Γ ∅ m_acc [] e;
+Definition to_while (e : expr Ti) (con bre : bool) (Ls : labelset) :
+    (labelset * option labelname * option labelname * (stmt Ti → stmt Ti)) :=
+  match con, bre with
+  | true, true =>
+     let Lc := fresh Ls in let Lb := fresh ({[ Lc ]} ∪ Ls) in
+     ({[ Lc ; Lb ]} ∪ Ls, Some Lc, Some Lb,
+      λ s, while{e} (s ;; label Lc) ;; label Lb)
+  | true, false =>
+     let Lc := fresh Ls in
+     ({[ Lc ]} ∪ Ls, Some Lc, None, λ s, while{e} (s ;; label Lc))
+  | false, true =>
+     let Lb := fresh Ls in
+     ({[ Lb ]} ∪ Ls, None, Some Lb, λ s, while{e} s ;; label Lb)
+  | false, false =>
+     (Ls, None, None, λ s, while{e} s)
+  end.
+Definition alloc_global (Γ : env Ti) (m : mem Ti) (xs : var_env Ti) (x : N)
+    (τ : type Ti) (mce : option (cexpr Ti)) : option (mem Ti * var_env Ti) :=
+  match mce with
+  | Some ce =>
+     '(e,τ') ← to_R <$> to_expr Γ ∅ m xs ce;
      guard (τ = τ');
      guard (int_typed (size_of Γ τ) sptrT);
-     v ← ⟦ e' ⟧ Γ ∅ [] m_acc ≫= maybe_inr;
-     go G (1 + o)%N (<[addr_top o τ:=v]{Γ}>(mem_alloc Γ o false τ m_acc))
-  | (τ,None) :: G =>
+     v ← ⟦ e ⟧ Γ ∅ [] m ≫= maybe_inr;
+     let o := fresh (dom _ m) in
+     Some (<[addr_top o τ:=v]{Γ}>(mem_alloc Γ o false τ m), (x,inl o) :: xs)
+  | None =>
      guard (✓{Γ} τ);
      guard (int_typed (size_of Γ τ) sptrT);
-     go G (1 + o)%N (<[addr_top o τ:=val_0 Γ τ]{Γ}>(mem_alloc Γ o false τ m_acc))
+     let o := fresh (dom _ m) in
+     Some (<[addr_top o τ:=val_0 Γ τ]{Γ}>(mem_alloc Γ o false τ m),
+           (x,inl o) :: xs)
   end.
-Definition to_funs (Γ : env Ti) (m : mem Ti) :
-    list (funname * list (type Ti) * type Ti * cstmt Ti) →
-    funmap (list (type Ti) * type Ti * stmt Ti) →
-    option (funmap (list (type Ti) * type Ti * stmt Ti)) :=
-  fix go Γfuns Γacc :=
-  match Γfuns with
-  | [] => Some Γacc
-  | (f,τs,σ,s) :: Γfuns =>
+
+Definition to_stmt (Γ : env Ti) (Γf : funtypes Ti) :
+    mem Ti → var_env Ti → labelset → option labelname → option labelname →
+    cstmt Ti → option (mem Ti * stmt Ti * rettype Ti) :=
+  fix go m xs Ls mLc mLb cs {struct cs} :=
+  match cs with
+  | SDo ce =>
+     '(e,_) ← to_R <$> to_expr Γ Γf m xs ce;
+     Some (m, !e, (false, None))
+  | SSkip => Some (m, skip, (false, None))
+  | SGoto l => Some (m, goto l, (true, None))
+  | SContinue => Lc ← mLc; Some (m, goto Lc, (true, None))
+  | SBreak => Lb ← mLb; Some (m, goto Lb, (true, None))
+  | SReturn (Some ce) =>
+     '(e,τ) ← to_R <$> to_expr Γ Γf m xs ce;
+     Some (m, ret e, (true, Some τ))
+  | SReturn None => Some (m, ret (#voidV), (true, Some voidT))
+  | SBlock x τ None cs =>
+     guard (✓{Γ} τ);
+     guard (int_typed (size_of Γ τ) sptrT);
+     '(m,s,cmσ) ← go m ((x,inr τ) :: xs) Ls mLc mLb cs;
+     Some (m, blk{τ} s, cmσ)
+  | SBlock x τ (Some ce) cs =>
+     guard (✓{Γ} τ);
+     guard (int_typed (size_of Γ τ) sptrT);
+     '(e,τ') ← to_R <$> to_expr Γ ∅ m ((x,inr τ) :: xs) ce;
+     guard (τ = τ');
+     '(m,s,cmσ) ← go m ((x,inr τ) :: xs) Ls mLc mLb cs;
+     Some (m, blk{τ} (var{τ} 0 ::= e ;; s), cmσ)
+  | SStatic x τ mce cs =>
+     '(m,xs) ← alloc_global Γ m xs x τ mce;
+     go m xs Ls mLc mLb cs
+  | SComp cs1 cs2 =>
+     '(m,s1,cmσ1) ← go m xs Ls mLc mLb cs1;
+     '(m,s2,cmσ2) ← go m xs Ls mLc mLb cs2;
+     mσ ← rettype_union (cmσ1.2) (cmσ2.2);
+     Some (m, s1 ;; s2, (cmσ2.1, mσ))
+  | SLabel l cs =>
+     '(m,s,cmσ) ← go m xs Ls mLc mLb cs; Some (m, l :; s, cmσ)
+  | SWhile ce cs =>
+     '(e,τ) ← to_R <$> to_expr Γ Γf m xs ce; _ ← maybe_TBase τ;
+     let '(Ls,mLc,mLb,Fs) :=
+       to_while e (cstmt_has_continue cs) (cstmt_has_break cs) Ls in
+     '(m,s,cmσ) ← go m xs Ls mLc mLb cs;
+     Some (m, Fs s, (false, cmσ.2))
+  | SIf ce cs1 cs2 =>
+     '(e,τ) ← to_R <$> to_expr Γ Γf m xs ce; _ ← maybe_TBase τ;
+     '(m,s1,cmσ1) ← go m xs Ls mLc mLb cs1;
+     '(m,s2,cmσ2) ← go m xs Ls mLc mLb cs2;
+     mσ ← rettype_union (cmσ1.2) (cmσ2.2);
+     Some (m, if{e} s1 else s2, (cmσ1.1 && cmσ2.1, mσ))%S
+  end%T.
+
+Fixpoint to_envs (Θ : list (N * decl Ti)) :
+    option (env Ti * funtypes Ti * funenv Ti * mem Ti * var_env Ti) :=
+  match Θ with
+  | [] => Some (∅,∅,∅,∅,[])
+  | (s,CompoundDecl τs) :: Θ =>
+     '(Γ,Γf,δ,m,xs) ← to_envs Θ;
+     let s : tag := s in
+     guard (Γ !! s = None);
+     guard (✓{Γ}* τs);
+     guard (1 < length τs);
+     Some (<[s:=τs]>Γ, Γf, δ, m, xs)
+  | (x,GlobDecl τ me) :: Θ =>
+     (* todo: we just shadow, that is wrong *)
+     '(Γ,Γf,δ,m,xs) ← to_envs Θ;
+     '(m,xs) ← alloc_global Γ m xs x τ me;
+      Some (Γ, Γf, δ, m, xs)
+  | (f,FunDecl ys σ cs) :: Θ =>
+     (* todo: functions and globals cannot have the same name *)
+     '(Γ,Γf,δ,m,xs) ← to_envs Θ;
+     let f : funname := f in
+     guard (NoDup (fst <$> ys));
+     let τs := snd <$> ys in
+     guard (Γf !! f = None);
      guard (✓{Γ}* τs);
      guard (Forall (λ τ, int_typed (size_of Γ τ) sptrT) τs);
-     '(s',cmσ) ← to_stmt Γ (fst <$> Γacc) m τs (labels s) None s;
+     let xs' := (prod_map id inr <$> ys) ++ xs in
+     '(m,s,cmσ) ← to_stmt Γ Γf m xs' (labels cs) None None cs;
      guard (rettype_match cmσ σ);
-     guard (Γacc !! f = None);
-     go Γfuns (<[f:=((τs,σ),s')]>Γacc)
+     Some(Γ, <[f:=(τs,σ)]>Γf, <[f:=s]>δ, m, xs)
   end.
-Definition to_envs (Θ : cenv Ti) :
-    option (env Ti * funtypes Ti * funenv Ti * mem Ti) :=
-  guard (list_env_valid (c_env Θ));
-  let Γ := map_of_list (c_env Θ) in
-  m ← to_mem Γ (c_globals Θ) 0%N ∅;
-  Fres ← to_funs Γ m (c_funs Θ) ∅;
-  Some (Γ, fst <$> Fres, snd <$> Fres, m).
 End frontend.
 
 Section cexpr_ind.
 Context {Ti : Set} (P : cexpr Ti → Prop).
-Context (Pvar : ∀ i, P (EVar i)).
-Context (Pglob : ∀ i, P (EGlob i)).
+Context (Pvar : ∀ x, P (EVar x)).
 Context (Pconst : ∀ τi x, P (EConst τi x)).
 Context (Paddrof : ∀ ce, P ce → P (EAddrOf ce)).
 Context (Pderef : ∀ ce, P ce → P (EDeref ce)).
@@ -279,21 +330,20 @@ Definition cexpr_ind_alt : ∀ e, P e :=
   fix go e :=
   match e return P e with
   | EVar _ => Pvar _
-  | EGlob _ => Pglob _
   | EConst _ _ => Pconst _ _
-  | EAddrOf ec => Paddrof _ (go ec)
-  | EDeref ec => Pderef _ (go ec)
-  | EAssign _ ec1 ec2 => Passign _ _ _ (go ec1) (go ec2)
-  | ECall f es => Pcall _ es $ list_ind (Forall P)
-       (Forall_nil_2 _) (λ e _, Forall_cons_2 _ _ _ (go e)) es
+  | EAddrOf ce => Paddrof _ (go ce)
+  | EDeref ce => Pderef _ (go ce)
+  | EAssign _ ce1 ce2 => Passign _ _ _ (go ce1) (go ce2)
+  | ECall f ces => Pcall _ ces $ list_ind (Forall P)
+      (Forall_nil_2 _) (λ ce _, Forall_cons_2 _ _ _ (go ce)) ces
   | EAlloc _ => Palloc _
-  | EFree ec => Pfree _ (go ec)
-  | EUnOp _ ec => Punop _ _ (go ec)
-  | EBinOp _ ec1 ec2 => Pbinop _ _ _ (go ec1) (go ec2)
-  | EIf ec1 ec2 ec3 => Pif _ _ _ (go ec1) (go ec2) (go ec3)
-  | EComma ec1 ec2 => Pcomma _ _ (go ec1) (go ec2)
-  | ECast _ ec => Pcast _ _ (go ec)
-  | EField ec _ => Pfield _ _ (go ec)
+  | EFree ce => Pfree _ (go ce)
+  | EUnOp _ ce => Punop _ _ (go ce)
+  | EBinOp _ ce1 ce2 => Pbinop _ _ _ (go ce1) (go ce2)
+  | EIf ce1 ce2 ce3 => Pif _ _ _ (go ce1) (go ce2) (go ce3)
+  | EComma ce1 ce2 => Pcomma _ _ (go ce1) (go ce2)
+  | ECast _ ce => Pcast _ _ (go ce)
+  | EField ce _ => Pfield _ _ (go ce)
   end.
 End cexpr_ind.
 
@@ -312,6 +362,20 @@ Implicit Types τlr : lrtype Ti.
 Arguments to_R _ _ : simpl never.
 Hint Extern 0 (_ ⊢ _ : _) => typed_constructor.
 
+Fixpoint var_env_stack_types (xs : var_env Ti) : list (type Ti) :=
+  match xs with
+  | [] => []
+  | (_,inr τ) :: xs => τ :: var_env_stack_types xs
+  | (_,inl _) :: xs => var_env_stack_types xs
+  end.
+Lemma var_env_stack_types_app xs1 xs2 :
+  var_env_stack_types (xs1 ++ xs2)
+  = var_env_stack_types xs1 ++ var_env_stack_types xs2.
+Proof. induction xs1 as [|[?[?|?]] ??]; f_equal'; auto. Qed.
+Lemma var_env_stack_types_snd (ys : list (N * type Ti)) :
+  var_env_stack_types (prod_map id inr <$> ys) = snd <$> ys.
+Proof. induction ys; f_equal'; auto. Qed.
+
 Lemma to_R_typed Γ Γf m τs e e' τlr τ' :
   to_R (e,τlr) = (e',τ') → (Γ,Γf,m,τs) ⊢ e : τlr → (Γ,Γf,m,τs) ⊢ e' : inr τ'.
 Proof.
@@ -320,14 +384,31 @@ Proof.
   { destruct τl; simplify_equality'. typed_constructor; eauto. }
   by typed_constructor.
 Qed.
-Lemma to_expr_typed Γ Γf m τs ce e τlr :
-  ✓ Γ → ✓{Γ} m → to_expr Γ Γf m τs ce = Some (e,τlr) → (Γ,Γf,m,τs) ⊢ e : τlr.
+Lemma var_lookup_typed Γ Γf m xs x e τ :
+  ✓ Γ → ✓{Γ} m → lookup_var m x 0 xs = Some (e,τ) →
+  (Γ,Γf,m,var_env_stack_types xs) ⊢ e : inl τ.
+Proof.
+  intros ??. cut (∀ τs', lookup_var m x (length τs') xs = Some (e,τ) →
+    (Γ,Γf,m,τs' ++ var_env_stack_types xs) ⊢ e : inl τ).
+  { intros help. apply (help []). }
+  induction xs as [|[x' [o|τ']] xs IH];
+    intros τs' ?; simplify_option_equality; eauto 2.
+  * typed_constructor; eauto using addr_top_typed, addr_top_strict,
+      index_typed_valid, index_typed_representable.
+  * typed_constructor. by rewrite list_lookup_middle.
+  * rewrite cons_middle, (associative_L (++)). apply (IH (τs' ++ [τ'])).
+    rewrite app_length; simpl. by rewrite Nat.add_comm.
+Qed.
+Lemma to_expr_typed Γ Γf m xs ce e τlr :
+  ✓ Γ → ✓{Γ} m → to_expr Γ Γf m xs ce = Some (e,τlr) →
+  (Γ,Γf,m,var_env_stack_types xs) ⊢ e : τlr.
 Proof.
   intros ??. assert (∀ ces eτlrs,
-     Forall (λ ce, ∀ e τlr,
-       to_expr Γ Γf m τs ce = Some (e,τlr) → (Γ,Γf,m,τs) ⊢ e : τlr) ces →
-     mapM (to_expr Γ Γf m τs) ces = Some eτlrs →
-     (Γ,Γf,m,τs) ⊢* fst <$> to_R <$> eτlrs :* inr <$> snd <$> to_R <$> eτlrs).
+     Forall (λ ce, ∀ e τlr, to_expr Γ Γf m xs ce = Some (e,τlr) →
+       (Γ,Γf,m,var_env_stack_types xs) ⊢ e : τlr) ces →
+     mapM (to_expr Γ Γf m xs) ces = Some eτlrs →
+     (Γ,Γf,m,var_env_stack_types xs) ⊢*
+       fst <$> to_R <$> eτlrs :* inr <$> snd <$> to_R <$> eτlrs).
   { intros ces eτlrs. rewrite mapM_Some. induction 2 as [|? [??]];
       decompose_Forall_hyps'; eauto using to_R_typed, surjective_pairing. }
   revert e τlr. induction ce using @cexpr_ind_alt; intros;
@@ -342,63 +423,89 @@ Proof.
     | H: binop_type_of _ _ _ = Some _ |- _ => apply binop_type_of_correct in H
     | _ => progress (simplify_option_equality by fail)
     | x : (_ * _)%type |- _ => destruct x
-    end; typed_constructor; eauto using to_R_typed,
-      index_typed_valid, index_typed_representable,
-      addr_top_typed, addr_top_strict.
+    end; try typed_constructor; eauto using to_R_typed, var_lookup_typed.
 Qed.
-Lemma to_stmt_typed Γ Γf m τs Ls mLcLb cs s cmτ :
-  ✓ Γ → ✓{Γ} m → to_stmt Γ Γf m τs Ls mLcLb cs = Some (s,cmτ) →
-  (Γ,Γf,m,τs) ⊢ s : cmτ.
+Lemma alloc_global_typed Γ m xs x τ mce m' xs' :
+  ✓ Γ → alloc_global Γ m xs x τ mce = Some (m',xs') →
+  ✓{Γ} m → ✓{Γ} m' ∧ (∀ o σ, m ⊢ o : σ → m' ⊢ o : σ)
+    ∧ var_env_stack_types xs = var_env_stack_types xs'.
 Proof.
-  intros ??. revert s cmτ τs Ls mLcLb. induction cs; intros;
+  assert (mem_allocable (fresh (dom indexset m)) m).
+  { eapply mem_allocable_alt, is_fresh. }
+  destruct mce as [ce|]; intros; simplify_equality'.
+  * destruct (to_expr Γ ∅ m xs ce) as [[e τlr]|] eqn:?; simplify_equality'.
+    destruct (to_R (e, τlr)) as [e' τ'] eqn:?.
+    repeat case_option_guard; simplify_equality'.
+    destruct (⟦ e' ⟧ Γ ∅ [] m) as [[?|v]|] eqn:?; simplify_equality'.
+    assert ((Γ,m) ⊢ inr v : inr τ'); [|typed_inversion_all].
+    { eapply (expr_eval_typed_aux Γ ∅ [] (var_env_stack_types xs) ∅);
+        eauto using to_R_typed, to_expr_typed, prefix_of_nil.
+      by intros ?; simpl_map. }
+    split; eauto using mem_alloc_val_valid, index_typed_alloc_val.
+  * repeat case_option_guard; simplify_equality'.
+    split; eauto using mem_alloc_val_valid, index_typed_alloc_val, val_0_typed.
+Qed.
+Lemma to_while_typed Γ Γf m τs e con bre Ls Ls' mLc mLb Fs s τb c mσ:
+  to_while e con bre Ls = (Ls',mLc,mLb,Fs) →
+  (Γ,Γf,m,τs) ⊢ e : inr (baseT τb) →
+  (Γ,Γf,m,τs) ⊢ s : (c,mσ) → (Γ,Γf,m,τs) ⊢ Fs s : (false,mσ).
+Proof.
+  destruct con, bre; intros; simplify_equality';
+    repeat typed_constructor; eauto using rettype_union_l.
+Qed.
+Lemma to_stmt_typed Γ Γf m xs Ls mLc mLb cs m' s cmτ :
+  ✓ Γ → ✓{Γ} m → to_stmt Γ Γf m xs Ls mLc mLb cs = Some (m',s,cmτ) →
+  (Γ,Γf,m',var_env_stack_types xs) ⊢ s : cmτ
+  ∧ ✓{Γ} m' ∧ (∀ o σ, m ⊢ o : σ → m' ⊢ o : σ).
+Proof.
+  intros ?. revert m m' s cmτ xs Ls mLc mLb. induction cs; intros;
     repeat match goal with
     | _ => case_match
     | _ : maybe_TBase ?τ = Some _ |- _ => is_var τ; destruct τ
     | _ => progress (simplify_option_equality by fail)
     | x : (_ * _)%type |- _ => destruct x
-    end; repeat typed_constructor;
-    eauto using to_R_typed, to_expr_typed, rettype_union_l; naive_solver.
+    | IH : ∀ _ _ _ _ _ _ _ _, ✓{Γ} _ → to_stmt _ _ _ _ _ _ _ ?cs = Some _ → _,
+      H : to_stmt _ _ _ _ _ _ _ ?cs = Some _ |- _ =>
+       destruct (λ Hm, IH _ _ _ _ _ _ _ _ Hm H) as (?&?&?); clear IH; [by auto|]
+    | H : to_expr _ _ _ _ _ = Some _ |- _ =>
+       apply to_expr_typed in H; [|by auto|by auto];
+       eapply to_R_typed in H; [|by eauto]
+    | H : alloc_global _ _ _ _ _ _ = Some _ |- _ =>
+       apply alloc_global_typed in H; [|by auto|by auto]; destruct H as (?&?&->)
+    end; try solve [split_ands; eauto using to_R_typed, to_expr_typed].
+  * split_ands; eauto. eapply SBlock_typed; eauto.
+    repeat typed_constructor; eauto using expr_typed_weaken, subseteq_empty.
+    constructor.
+  * split_ands; eauto using stmt_typed_weaken.
+  * split_ands; eauto using to_while_typed, expr_typed_weaken.
+  * split_ands; eauto using stmt_typed_weaken, expr_typed_weaken.
 Qed.
-Lemma to_mem_typed Γ τmes o m m' :
-  ✓ Γ → to_mem Γ τmes o m = Some m' → ✓{Γ} m → 
-  (∀ o', (o ≤ o')%N → mem_allocable o' m) → ✓{Γ} m'.
+Lemma to_envs_typed Θ Γ Γf δ m xs :
+  to_envs Θ = Some (Γ,Γf,δ,m,xs) →
+  ✓ Γ ∧ (Γ,m) ⊢ δ : Γf ∧ ✓{Γ} m ∧ var_env_stack_types xs = [].
 Proof.
-  intros ?. revert m o m'. induction τmes as [|[τ [ce|]] τmes IH];
-    intros m o m' ???; simplify_equality'; auto.
-  * destruct (to_expr Γ ∅ m [] ce) as [[e τlr]|] eqn:?; simplify_equality'.
-    destruct (to_R (e, τlr)) as [e' τ'] eqn:?.
+  revert Γ Γf δ m xs. induction Θ as [|[x [τs|τ mce|ys σ cs]] Θ IH];
+    intros Γ Γf δ m xs ?; simplify_equality'.
+  * eauto using env_empty_valid, cmap_empty_valid.
+  * destruct (to_envs Θ) as [[[[[Γ2 ?] ?] ?] ?]|]; simplify_option_equality.
+    destruct (IH Γ2 Γf δ m xs) as (?&?&?&?); eauto. split_ands; auto.
+    + by constructor.
+    + eapply funenv_typed_weaken; eauto using insert_subseteq.
+    + eapply cmap_valid_weaken; eauto using insert_subseteq.
+  * destruct (to_envs Θ) as [[[[[Γ2 Γf2] δ2] m2] xs2]|]; simplify_equality'.
+    destruct (alloc_global _ _ _ _ _ _) as [[??]|] eqn:?; simplify_equality'.
+    destruct (IH Γ Γf δ m2 xs2) as (?&?&?&?); eauto.
+    destruct (alloc_global_typed Γ m2 xs2 x τ mce m xs)
+      as (?&?&<-); eauto using funenv_typed_weaken.
+  * destruct (to_envs Θ) as [[[[[Γ2 Γf2] δ2] m2] xs2]|]; simplify_equality'.
     repeat case_option_guard; simplify_equality'.
-    destruct (⟦ e' ⟧ Γ ∅ [] m) as [[?|v]|] eqn:?; simplify_equality'.
-    assert ((Γ,m) ⊢ inr v : inr τ'); [|typed_inversion_all].
-    { eapply expr_eval_typed; eauto using to_R_typed, to_expr_typed.
-      by intros ?; simplify_map_equality'. }
-    eapply IH; eauto using mem_alloc_val_valid.
-    intros; eapply mem_alloc_val_allocable. eauto with lia. intros ->; lia.
-  * repeat case_option_guard; simplify_equality'.
-    eapply IH; eauto using mem_alloc_val_valid, val_0_typed.
-    intros; eapply mem_alloc_val_allocable. eauto with lia. intros ->; lia.
-Qed.
-Lemma to_funs_typed Γ m Γfuns Γacc Γres :
-  ✓ Γ → ✓{Γ} m → to_funs Γ m Γfuns Γacc = Some Γres →
-  (Γ,m) ⊢ snd <$> Γacc : fst <$> Γacc → (Γ,m) ⊢ snd <$> Γres : fst <$> Γres.
-Proof.
-  intros ??. revert Γres Γacc. induction Γfuns as [|[[[f τs] τ] cs] Γfuns IH];
-    intros Γres Γacc ??; simplify_equality'; auto.
-  repeat case_option_guard; simplify_equality'.
-  destruct (to_stmt _ _ _ _ _ _ _) as [[s mτ]|] eqn:?; simplify_equality'.
-  repeat case_option_guard; simplify_equality'.
-  eapply IH; eauto. rewrite !fmap_insert; simpl; typed_constructor; eauto.
-  * by rewrite lookup_fmap; simplify_option_equality.
-  * eauto using to_stmt_typed.
-Qed.
-Lemma to_envs_typed Θ Γ Γf δ m :
-  to_envs Θ = Some (Γ,Γf,δ,m) → ✓ Γ ∧ (Γ,m) ⊢ δ : Γf ∧ ✓{Γ} m.
-Proof.
-  unfold to_envs; intros; simplify_option_equality.
-  assert (✓ (map_of_list (c_env Θ))) by eauto using env_valid_of_list.
-  assert (✓{map_of_list (c_env Θ)} m)
-    by eauto using to_mem_typed, cmap_empty_valid, mem_empty_allocable.
-  split_ands; auto; eapply to_funs_typed; eauto.
-  rewrite !fmap_empty. by typed_constructor.
+    destruct (to_stmt _ _ _ _ _ _ _ _)
+      as [[[m3 s] cmσ]|] eqn:?; simplify_option_equality.
+    destruct (IH Γ Γf2 δ2 m2 xs) as (?&?&?&Hxs); eauto.
+    destruct (to_stmt_typed Γ Γf2 m2 ((prod_map id inr <$> ys) ++ xs)
+      (labels cs) None None cs m s cmσ) as (Hs&?&?); auto.
+    rewrite var_env_stack_types_app,
+      var_env_stack_types_snd, Hxs, (right_id_L [] (++)) in Hs.
+    split_ands; eauto using funenv_typed_weaken.
 Qed.
 End properties.
